src/cddl/pulse/CDDL.Pulse.Serialize.Gen.MapGroup.ZeroOrMore.Aux2.Lemma13.fsti
@@ -1,0 +1,37 @@
+module CDDL.Pulse.Serialize.Gen.MapGroup.ZeroOrMore.Aux2.Lemma13
+include CDDL.Pulse.Serialize.Gen.MapGroup.ZeroOrMore.Aux2.Invariant
+
+module S = Pulse.Lib.Slice
+module U8 = FStar.UInt8
+module SZ = FStar.SizeT
+module U64 = FStar.UInt64
+module Map = CDDL.Spec.Map
+
+val invariant_insert_dup
+  (#pe: cbor_parser)
+  (#minl: cbor_min_length pe)
+  (#maxl: cbor_max_length pe)
+  (p: cbor_map_parser minl maxl)
+  (key: typ) (tkey: Type0)
+  (sp1: spec key tkey true)
+  (value: typ) (tvalue: Type0)
+  (inj: bool)
+  (sp2: spec value tvalue inj)
+  (except: map_constraint { inj \/ map_constraint_value_injective key sp2.parser except })
+  (em: bool)
+  (out: S.slice U8.t)
+  (vout: Seq.seq U8.t)
+  (size: SZ.t)
+  (count: U64.t)
+  (m: cbor_map)
+  (v0 v: Map.t tkey (list tvalue))
+  (min: nat)
+  (max: option nat)
+: Lemma
+  (requires
+    impl_serialize_map_zero_or_more_iterator_gen_invariant_min p sp1 sp2 except min v0 v /\
+    impl_serialize_map_zero_or_more_iterator_gen_invariant_max p sp1 sp2 except max v0 v
+  )
+  (ensures
+    impl_serialize_map_zero_or_more_iterator_gen_invariant p sp1 sp2 except em out vout size count m v0 v min max false
+  )
